@prefix : <http://purl.org/heo#> .
@prefix owl: <http://www.w3.org/2002/07/owl#> .
@prefix rdf: <http://www.w3.org/1999/02/22-rdf-syntax-ns#> .
@prefix xml: <http://www.w3.org/XML/1998/namespace> .
@prefix xsd: <http://www.w3.org/2001/XMLSchema#> .
@prefix rdfs: <http://www.w3.org/2000/01/rdf-schema#> .
@base <http://purl.org/heo> .

<http://purl.org/heo> rdf:type owl:Ontology ;
                       owl:versionInfo "Version 0.2"^^xsd:string .

#################################################################
#    Annotation properties
#################################################################

###  http://attempto.ifi.uzh.ch/ace_lexicon#CN_pl
<http://attempto.ifi.uzh.ch/ace_lexicon#CN_pl> rdf:type owl:AnnotationProperty .


###  http://attempto.ifi.uzh.ch/ace_lexicon#CN_sg
<http://attempto.ifi.uzh.ch/ace_lexicon#CN_sg> rdf:type owl:AnnotationProperty .


###  http://attempto.ifi.uzh.ch/ace_lexicon#TV_pl
<http://attempto.ifi.uzh.ch/ace_lexicon#TV_pl> rdf:type owl:AnnotationProperty .


###  http://attempto.ifi.uzh.ch/ace_lexicon#TV_sg
<http://attempto.ifi.uzh.ch/ace_lexicon#TV_sg> rdf:type owl:AnnotationProperty .


###  http://attempto.ifi.uzh.ch/ace_lexicon#TV_vbg
<http://attempto.ifi.uzh.ch/ace_lexicon#TV_vbg> rdf:type owl:AnnotationProperty .


###  http://purl.org/heo#expressedBy
:expressedBy rdf:type owl:AnnotationProperty ;
             rdfs:comment "Indicates that the reference points to observable behavior expressing the emotion."^^xsd:string ;
             rdfs:label "expressed by"^^xsd:string ;
             rdfs:domain :Emotion .


###  http://purl.org/heo#expressedThrough
:expressedThrough rdf:type owl:AnnotationProperty ;
                  rdfs:comment "The modality, or list of modalities, through which the emotion is expressed. An attribute of type xsd:NMTOKENS which contains a space delimited set of values from an open set of values including: {gaze, face, head, torso, gesture, leg, voice, text, locomotion, posture, physiology, ...}."^^xsd:string ;
                  rdfs:label "expressed through"^^xsd:string ;
                  rdfs:domain :Emotion .


###  http://purl.org/heo#targetedAt
:targetedAt rdf:type owl:AnnotationProperty ;
            rdfs:comment "Indicates that the reference points to an object towards which an emotion-related action, or action tendency, is directed."^^xsd:string ;
            rdfs:label "targeted at"^^xsd:string ;
            rdfs:domain :Emotion .


###  http://purl.org/heo#triggeredBy
:triggeredBy rdf:type owl:AnnotationProperty ;
             rdfs:comment "Indicates that the reference points to an emotion-eliciting event that caused an emotion and/or related appraisals"^^xsd:string ;
             rdfs:label "triggered by"^^xsd:string ;
             rdfs:domain :Emotion .


#################################################################
#    Data properties
#################################################################

###  http://purl.org/heo#intensity
:intensity rdf:type owl:DatatypeProperty ;
           rdfs:range [ rdf:type rdfs:Datatype ;
                        owl:onDatatype xsd:float ;
                        owl:withRestrictions ( [ xsd:minExclusive "0.0"^^xsd:float
                                               ]
                                               [ xsd:maxExclusive "1.0"^^xsd:float
                                               ]
                                             )
                      ] .


#################################################################
#    Classes
#################################################################

###  http://purl.org/heo#ActionTendency
:ActionTendency rdf:type owl:Class ;
                <http://attempto.ifi.uzh.ch/ace_lexicon#CN_pl> "ActionTendencies"^^xsd:string ;
                <http://attempto.ifi.uzh.ch/ace_lexicon#CN_sg> "ActionTendency"^^xsd:string ;
                rdfs:comment "Emotions have a strong influence on the motivational state of a subject. Emotion theory associates emotions to a small set of so-called action tendencies, e.g. avoidance (relates to fear), rejecting (disgust) etc. Action tendencies can be viewed as a link between the outcome of an appraisal process and actual actions."^^xsd:string ;
                rdfs:label "Action Tendency"^^xsd:string .


###  http://purl.org/heo#Agonistic
:Agonistic rdf:type owl:Class ;
           rdfs:subClassOf :Frijda_Action_Tendency ;
           <http://attempto.ifi.uzh.ch/ace_lexicon#CN_pl> "Agonistics"^^xsd:string ;
           <http://attempto.ifi.uzh.ch/ace_lexicon#CN_sg> "Agonistic"^^xsd:string ;
           rdfs:comment "Agonistic (FrijdaActionTendency ) [aimed at removal of obstruction and regaining control, related to anger]"^^xsd:string ;
           rdfs:label "Agonistic"^^xsd:string .


###  http://purl.org/heo#Appraisal_Model
:Appraisal_Model rdf:type owl:Class ;
                 <http://attempto.ifi.uzh.ch/ace_lexicon#CN_pl> "Appraisals"^^xsd:string ;
                 <http://attempto.ifi.uzh.ch/ace_lexicon#CN_sg> "Appraisal"^^xsd:string ;
                 rdfs:comment "The term \"appraisal\" is used in the scientific literature to describe the evaluation process leading to an emotional response. Triggered by an \"emotion-eliciting event\", an individual carries out an automatic, subjective assessment of the event, in order to determine the relevance of the event to the individual. This assessment is carried out along a number of \"appraisal dimensions\" such as the novelty, pleasantness or goal conduciveness of the event."^^xsd:string ;
                 rdfs:label "Appraisal_Model - Componential  Model-"^^xsd:string .


###  http://purl.org/heo#Approach
:Approach rdf:type owl:Class ;
          rdfs:subClassOf :Frijda_Action_Tendency ;
          <http://attempto.ifi.uzh.ch/ace_lexicon#CN_pl> "Approaches"^^xsd:string ;
          <http://attempto.ifi.uzh.ch/ace_lexicon#CN_sg> "Approach"^^xsd:string ;
          rdfs:comment "Approach (FrijdaActionTendency ) [aimed towards access and consummatory activity, related to desire]"^^xsd:string ;
          rdfs:label "Approach"^^xsd:string .


###  http://purl.org/heo#Attending
:Attending rdf:type owl:Class ;
           rdfs:subClassOf :Frijda_Action_Tendency ;
           <http://attempto.ifi.uzh.ch/ace_lexicon#CN_pl> "Attendings"^^xsd:string ;
           <http://attempto.ifi.uzh.ch/ace_lexicon#CN_sg> "Attending"^^xsd:string ;
           rdfs:comment "Attending (FrijdaActionTendency ) [aimed at identification, related to interest]"^^xsd:string ;
           rdfs:label "Attending"^^xsd:string .


###  http://purl.org/heo#Avoidance
:Avoidance rdf:type owl:Class ;
           rdfs:subClassOf :Frijda_Action_Tendency ;
           <http://attempto.ifi.uzh.ch/ace_lexicon#CN_pl> "Avoidances"^^xsd:string ;
           <http://attempto.ifi.uzh.ch/ace_lexicon#CN_sg> "Avoidance"^^xsd:string ;
           rdfs:comment "Avoidance (FrijdaActionTendency ) [aimed towards own inaccessibility and protection, related to fear]"^^xsd:string ;
           rdfs:label "Avoidance"^^xsd:string .


###  http://purl.org/heo#Being-with
:Being-with rdf:type owl:Class ;
            rdfs:subClassOf :Frijda_Action_Tendency ;
            <http://attempto.ifi.uzh.ch/ace_lexicon#CN_pl> "Being-withs"^^xsd:string ;
            <http://attempto.ifi.uzh.ch/ace_lexicon#CN_sg> "Being-with"^^xsd:string ;
            rdfs:comment "Being with (FrijdaActionTendency ) [aimed at contact and interaction, related to enjoyment]"^^xsd:string ;
            rdfs:label "Being with"^^xsd:string .


###  http://purl.org/heo#Dominating
:Dominating rdf:type owl:Class ;
            rdfs:subClassOf :Frijda_Action_Tendency ;
            <http://attempto.ifi.uzh.ch/ace_lexicon#CN_pl> "Dominatings"^^xsd:string ;
            <http://attempto.ifi.uzh.ch/ace_lexicon#CN_sg> "Dominating"^^xsd:string ;
            rdfs:comment "Dominating (FrijdaActionTendency ) [aimed at retained control, related to arrogance]"^^xsd:string ;
            rdfs:label "Dominating"^^xsd:string .


###  http://purl.org/heo#Frijda_Action_Tendency
:Frijda_Action_Tendency rdf:type owl:Class ;
                        rdfs:subClassOf :ActionTendency ;
                        <http://attempto.ifi.uzh.ch/ace_lexicon#CN_pl> "FrijdaActionTendencies"^^xsd:string ;
                        <http://attempto.ifi.uzh.ch/ace_lexicon#CN_sg> "FrijdaActionTendency"^^xsd:string ;
                        rdfs:comment "An action tendency defined by Nico Frijda, who also coined the term 'action tendency'"^^xsd:string .


###  http://purl.org/heo#Interrupting
:Interrupting rdf:type owl:Class ;
              rdfs:subClassOf :Frijda_Action_Tendency ;
              <http://attempto.ifi.uzh.ch/ace_lexicon#CN_pl> "Interruptings"^^xsd:string ;
              <http://attempto.ifi.uzh.ch/ace_lexicon#CN_sg> "Interrupting"^^xsd:string ;
              rdfs:comment "Interrupting (FrijdaActionTendency ) [aimed at reorientation, related to shock and surprise]"^^xsd:string ;
              rdfs:label "Interrupting"^^xsd:string .


###  http://purl.org/heo#Nonattending
:Nonattending rdf:type owl:Class ;
              rdfs:subClassOf :Frijda_Action_Tendency ;
              <http://attempto.ifi.uzh.ch/ace_lexicon#CN_pl> "Nonattendings"^^xsd:string ;
              <http://attempto.ifi.uzh.ch/ace_lexicon#CN_sg> "Nonattending"^^xsd:string ;
              rdfs:comment "Nonattending (FrijdaActionTendency ) [aimed at selecting, related to indifference]"^^xsd:string ;
              rdfs:label "Nonattending"^^xsd:string .


###  http://purl.org/heo#OCCAppraisalAppealingness
:OCCAppraisalAppealingness rdf:type owl:Class ;
                           rdfs:subClassOf :OCC_Appraisal ;
                           <http://attempto.ifi.uzh.ch/ace_lexicon#CN_pl> "OCCAppraisalAppealingnesses"^^xsd:string ;
                           <http://attempto.ifi.uzh.ch/ace_lexicon#CN_sg> "OCCAppraisalAppealingness"^^xsd:string ;
                           rdfs:comment "Appealingness (OCCAppraisal)  [relevant for attraction emotions. (liking/disliking)]"^^xsd:string ;
                           rdfs:label "Appealingness"^^xsd:string .


###  http://purl.org/heo#OCCAppraisalDeservingness
:OCCAppraisalDeservingness rdf:type owl:Class ;
                           rdfs:subClassOf :OCC_Appraisal ;
                           <http://attempto.ifi.uzh.ch/ace_lexicon#CN_pl> "OCCAppraisalDeservingnesses"^^xsd:string ;
                           <http://attempto.ifi.uzh.ch/ace_lexicon#CN_sg> "OCCAppraisalDeservingness"^^xsd:string ;
                           rdfs:comment "Deservingness (OCCAppraisal)  [related to fortunes of others. Whether the other “deserves” the event.]"^^xsd:string ;
                           rdfs:label "Deservingness"^^xsd:string .


###  http://purl.org/heo#OCCAppraisalDesirability
:OCCAppraisalDesirability rdf:type owl:Class ;
                          rdfs:subClassOf :OCC_Appraisal ;
                          <http://attempto.ifi.uzh.ch/ace_lexicon#CN_pl> "OCCAppraisalDesirabilities"^^xsd:string ;
                          <http://attempto.ifi.uzh.ch/ace_lexicon#CN_sg> "OCCAppraisalDesirability"^^xsd:string ;
                          rdfs:comment "Desirability (OCCAppraisal)  [relevant for event based emotions. (pleased/displeased)]"^^xsd:string ;
                          rdfs:label "Desirability"^^xsd:string .


###  http://purl.org/heo#OCCAppraisalDesirability-for-other
:OCCAppraisalDesirability-for-other rdf:type owl:Class ;
                                    rdfs:subClassOf :OCC_Appraisal ;
                                    <http://attempto.ifi.uzh.ch/ace_lexicon#CN_pl> "OCCAppraisalDesirability-for-others"^^xsd:string ;
                                    <http://attempto.ifi.uzh.ch/ace_lexicon#CN_sg> "OCCAppraisalDesirability-for-other"^^xsd:string ;
                                    rdfs:comment "Desirability-for-other (OCCAppraisal)  [related to fortunes of others. Whether the event is desirable for the other.]"^^xsd:string ;
                                    rdfs:label "Desirability for other"^^xsd:string .


###  http://purl.org/heo#OCCAppraisalEffort
:OCCAppraisalEffort rdf:type owl:Class ;
                    rdfs:subClassOf :OCC_Appraisal ;
                    <http://attempto.ifi.uzh.ch/ace_lexicon#CN_pl> "OCCAppraisalEfforts"^^xsd:string ;
                    <http://attempto.ifi.uzh.ch/ace_lexicon#CN_sg> "OCCAppraisalEffort"^^xsd:string ;
                    rdfs:comment "Effort (OCCAppraisal)  [relevant for prospect emotions. How much effort the individual invested in the outcome.]"^^xsd:string ;
                    rdfs:label "Effort"^^xsd:string .


###  http://purl.org/heo#OCCAppraisalExpectation-of-deviation
:OCCAppraisalExpectation-of-deviation rdf:type owl:Class ;
                                      rdfs:subClassOf :OCC_Appraisal ;
                                      <http://attempto.ifi.uzh.ch/ace_lexicon#CN_pl> "OCCAppraisalExpectation-of-deviations"^^xsd:string ;
                                      <http://attempto.ifi.uzh.ch/ace_lexicon#CN_sg> "OCCAppraisalExpectation-of-deviation"^^xsd:string ;
                                      rdfs:comment "Expectation-of-deviation (OCCAppraisal)  [relevant for attribution emotions. Distinguishes whether the other is expected to act in the manner deserving of admiration or reproach. These distinguish b between: pride, shame, admiration, reproach.]"^^xsd:string ;
                                      rdfs:label "Expectation of deviation"^^xsd:string .


###  http://purl.org/heo#OCCAppraisalFamiliarity
:OCCAppraisalFamiliarity rdf:type owl:Class ;
                         rdfs:subClassOf :OCC_Appraisal ;
                         <http://attempto.ifi.uzh.ch/ace_lexicon#CN_pl> "OCCAppraisalFamiliarities"^^xsd:string ;
                         <http://attempto.ifi.uzh.ch/ace_lexicon#CN_sg> "OCCAppraisalFamiliarity"^^xsd:string ;
                         rdfs:comment "Familiarity (OCCAppraisal)  [relevant for attraction emotions. (love/hate)]"^^xsd:string ;
                         rdfs:label "Familiarity"^^xsd:string .


###  http://purl.org/heo#OCCAppraisalLikelihood
:OCCAppraisalLikelihood rdf:type owl:Class ;
                        rdfs:subClassOf :OCC_Appraisal ;
                        <http://attempto.ifi.uzh.ch/ace_lexicon#CN_pl> "OCCAppraisalLikelihoods"^^xsd:string ;
                        <http://attempto.ifi.uzh.ch/ace_lexicon#CN_sg> "OCCAppraisalLikelihood"^^xsd:string ;
                        rdfs:comment "Likelihood (OCCAppraisal)  [relevant for prospect emotions. (hope/fear)]"^^xsd:string ;
                        rdfs:label "Likelihood"^^xsd:string .


###  http://purl.org/heo#OCCAppraisalLiking
:OCCAppraisalLiking rdf:type owl:Class ;
                    rdfs:subClassOf :OCC_Appraisal ;
                    <http://attempto.ifi.uzh.ch/ace_lexicon#CN_pl> "OCCAppraisalLikings"^^xsd:string ;
                    <http://attempto.ifi.uzh.ch/ace_lexicon#CN_sg> "OCCAppraisalLiking"^^xsd:string ;
                    rdfs:comment "Liking (OCCAppraisal)  [related to fortunes of others. Whether the other is liked or not. These distinguish between: happy-for, pity, gloating (schadenfreude), and resentment.]"^^xsd:string ;
                    rdfs:label "Liking"^^xsd:string .


###  http://purl.org/heo#OCCAppraisalPraiseworthiness
:OCCAppraisalPraiseworthiness rdf:type owl:Class ;
                              rdfs:subClassOf :OCC_Appraisal ;
                              <http://attempto.ifi.uzh.ch/ace_lexicon#CN_pl> "OCCAppraisalPraiseworthinesses"^^xsd:string ;
                              <http://attempto.ifi.uzh.ch/ace_lexicon#CN_sg> "OCCAppraisalPraiseworthiness"^^xsd:string ;
                              rdfs:comment "Praiseworthiness (OCCAppraisal)  [relevant for attribution emotions. (approving/disapproving)]"^^xsd:string ;
                              rdfs:label "Praiseworthiness"^^xsd:string .


###  http://purl.org/heo#OCCAppraisalRealization
:OCCAppraisalRealization rdf:type owl:Class ;
                         rdfs:subClassOf :OCC_Appraisal ;
                         <http://attempto.ifi.uzh.ch/ace_lexicon#CN_pl> "OCCAppraisalRealizations"^^xsd:string ;
                         <http://attempto.ifi.uzh.ch/ace_lexicon#CN_sg> "OCCAppraisalRealization"^^xsd:string ;
                         rdfs:comment "Realization (OCCAppraisal)  [relevant for prospect emotions. The actual resulting outcome. These distinguish between: relief, disappointment, satisfaction, and fears-confirmed.]"^^xsd:string ;
                         rdfs:label "Realization"^^xsd:string .


###  http://purl.org/heo#OCCAppraisalStrength-of-identification
:OCCAppraisalStrength-of-identification rdf:type owl:Class ;
                                        rdfs:subClassOf :OCC_Appraisal ;
                                        <http://attempto.ifi.uzh.ch/ace_lexicon#CN_pl> "OCCAppraisalStrength-of-identifications"^^xsd:string ;
                                        <http://attempto.ifi.uzh.ch/ace_lexicon#CN_sg> "OCCAppraisalStrength-of-identification"^^xsd:string ;
                                        rdfs:comment "Strength-of-identification (OCCAppraisal)  [relevant for attribution emotions. The stronger one identifies with the other, that distinguishes between whether pride or admiration is felt.]"^^xsd:string ;
                                        rdfs:label "Strength of identification"^^xsd:string .


###  http://purl.org/heo#OCC_Appraisal
:OCC_Appraisal rdf:type owl:Class ;
               rdfs:subClassOf :Appraisal_Model ;
               <http://attempto.ifi.uzh.ch/ace_lexicon#CN_sg> "OCCAppraisal"^^xsd:string .


###  http://purl.org/heo#Rejecting
:Rejecting rdf:type owl:Class ;
           rdfs:subClassOf :Frijda_Action_Tendency ;
           <http://attempto.ifi.uzh.ch/ace_lexicon#CN_pl> "Rejectings"^^xsd:string ;
           <http://attempto.ifi.uzh.ch/ace_lexicon#CN_sg> "Rejecting"^^xsd:string ;
           rdfs:comment "Rejecting (FrijdaActionTendency ) [aimed at removal of object, related to disgust]"^^xsd:string ;
           rdfs:label "Rejecting"^^xsd:string .


###  http://purl.org/heo#Submitting
:Submitting rdf:type owl:Class ;
            rdfs:subClassOf :Frijda_Action_Tendency ;
            <http://attempto.ifi.uzh.ch/ace_lexicon#CN_pl> "Submittings"^^xsd:string ;
            <http://attempto.ifi.uzh.ch/ace_lexicon#CN_sg> "Submitting"^^xsd:string ;
            rdfs:comment "Submitting (FrijdaActionTendency ) [aimed at deflecting pressure, related to humility and resignation]"^^xsd:string ;
            rdfs:label "Submitting"^^xsd:string .


###  Generated by the OWL API (version 5.1.0) https://github.com/owlcs/owlapi/
